Narrow down the holes in weak mark lemmas. The proof strategy used there is very useful. And, for now, accidentally, we do not depend on any decidability premise in these weak mark lemmas.

graph/weak_mark_lemmas.v
@@ -77,8 +77,7 @@ Definition nothing (n : V) (g1 : Graph) (g2 : Graph) : Prop :=
 Definition mark1 (n : V) (g1 : Graph) (g2 : Graph) : Prop :=
   g1 ~=~ g2 /\
   marked g2 n /\
-  (forall n', n <> n' -> vvalid g1 n' -> vvalid g2 n' -> vlabel g1 n' = vlabel g2 n') /\
-  (forall e, evalid g1 e -> evalid g2 e -> elabel g1 e = elabel g2 e).
+  (forall n', n <> n' -> (marked g1 n' <-> marked g2 n')).
 
 Definition mark (root : V) (g1 : Graph) (g2 : Graph) : Prop :=
   let PV := reachable_by g1 root (unmarked g1) in
@@ -103,6 +102,27 @@ Proof.
   intro.
   apply reachable_by_foot_prop in H1.
   unfold unmarked in H1; rewrite negateP_spec in H1; auto.
+Qed.
+
+Lemma mark_unmarked: forall (g1: Graph) root (g2: Graph),
+  mark root g1 g2 ->
+  Same_set (unmarked g2) (Intersection _ (unmarked g1) (Complement _ (reachable_by g1 root (unmarked g1)))).
+Proof.
+  intros.
+  rewrite Same_set_spec; intro n.
+  rewrite Intersection_spec; unfold Complement, Ensembles.In.
+  pose proof H.
+  destruct H as [_ [? ?]].
+  specialize (H n); specialize (H1 n).
+  unfold unmarked at 1 2; rewrite !negateP_spec.
+  split; intros; [split |].
+  + intro; apply H2; clear H2.
+    eapply mark_marked; eauto.
+  + intro; apply H2; clear H2.
+    apply H; auto.
+  + destruct H2.
+    apply H1 in H3.
+    tauto.
 Qed.
 
 Lemma mark_invalid_refl: forall (g: Graph) root, ~ vvalid g root -> mark root g g.
@@ -175,8 +195,7 @@ Lemma mark1_componded_mark_list_mark: forall root l (g1 g2: Graph)
   mark root g1 g2.
 Abort.
 
-Lemma triple1_mark: forall (g g1 g2: Graph) root l l_done son l_later
-  (V_DEC: forall x, In x l -> Decidable (vvalid g1 x)),
+Lemma triple1_mark: forall (g g1 g2: Graph) root l l_done son l_later,
   vvalid g root ->
   (unmarked g) root ->
   let unmarked' := Intersection _ (unmarked g) (Complement _ (eq root)) in
@@ -208,8 +227,95 @@ Proof.
     apply Included_refl.
 Qed.
 
-Lemma mark1_mark_list_mark: forall root l (g1 g2: Graph)
-  (V_DEC: forall x, In x l -> Decidable (vvalid g1 x)),
+Lemma triple2_mark: forall (g g1 g2: Graph) root l l_done son l_later,
+  vvalid g root ->
+  (unmarked g) root ->
+  let unmarked' := Intersection _ (unmarked g) (Complement _ (eq root)) in
+  step_list g root l ->
+  l = l_done ++ son :: l_later ->
+  let PV1 := reachable_by_through_set g l_done unmarked' in
+  (predicate_partialgraph g (Complement _ PV1)) ~=~ (predicate_partialgraph g1 (Complement _ PV1)) /\
+  Same_set (unmarked g1) (Intersection _ unmarked' (Complement _ PV1)) ->
+  mark son g1 g2 ->
+  let PV2 := reachable_by_through_set g (l_done ++ son :: nil) unmarked' in
+  Same_set (unmarked g2) (Intersection _ unmarked' (Complement _ PV2)).
+Proof.
+  intros.
+  destruct H3 as [PRE_psi PRE_unm].
+  apply mark_unmarked in H4.
+  rewrite H4, PRE_unm.
+  rewrite (Intersection_comm _ unmarked') at 2.
+  rewrite reachable_by_eq_partialgraph_reachable', <- partial_partialgraph, <- PRE_psi, <- reachable_by_eq_partialgraph_reachable'.
+  unfold PV2.
+  rewrite Complement_reachable_by_through_app_strong, reachable_by_through_singleton'.
+  rewrite Intersection_assoc.
+  reflexivity.
+Qed.  
+
+Lemma triple_mark1: forall root (g g1: Graph),
+  mark1 root g g1 ->
+  let unmarked' := Intersection _ (unmarked g) (Complement _ (eq root)) in
+  let PV1 := reachable_by_through_set g nil unmarked' in
+  (predicate_partialgraph g (Complement _ PV1)) ~=~ (predicate_partialgraph g1 (Complement _ PV1)) /\
+  Same_set (unmarked g1) (Intersection _ unmarked' (Complement _ PV1)).
+Proof.
+  intros.
+  split.
+  + destruct H.
+    rewrite H; reflexivity.
+  + unfold PV1, unmarked'.
+    rewrite Same_set_spec; intro n; rewrite !Intersection_spec.
+    unfold Complement, Ensembles.In.
+    rewrite reachable_by_through_nil.
+    destruct H as [_ [? ?]].
+    unfold unmarked; rewrite !negateP_spec.
+    destruct_eq_dec root n.
+    - subst n; tauto.
+    - specialize (H0 n).
+      tauto.
+Qed.
+
+Lemma triple_final: forall root l (g g1: Graph),
+  vvalid g root ->
+  (unmarked g) root ->
+  step_list g root l ->
+  let unmarked' := Intersection _ (unmarked g) (Complement _ (eq root)) in
+  let PV1 := reachable_by_through_set g l unmarked' in
+  (predicate_partialgraph g (Complement _ PV1)) ~=~ (predicate_partialgraph g1 (Complement _ PV1)) /\
+  Same_set (unmarked g1) (Intersection _ unmarked' (Complement _ PV1)) ->
+  mark root g g1.
+Proof.
+  intros.
+  destruct H2.
+  assert (Same_set (reachable_by g root (unmarked g)) (Union _ (eq root) PV1)).
+  Focus 1. {
+    rewrite Same_set_spec.
+    intro. rewrite Union_spec.
+    apply reachable_by_step_equiv; auto.
+  } Unfocus.
+  split; [| split].
+  + eapply si_stronger_partialgraph_simple; [| exact H2].
+    apply Complement_Included_rev.
+    rewrite H4.
+    apply right_Included_Union.
+  + intros.
+    rewrite Same_set_spec in H4; rewrite (H4 n), Union_spec in H5.
+    rewrite Same_set_spec in H3; specialize (H3 n).
+    rewrite Intersection_spec in H3.
+    unfold unmarked', unmarked, Complement, Ensembles.In in H3.
+    rewrite Intersection_spec, !negateP_spec in H3.
+    destruct (node_pred_dec (marked g1) n); auto.
+    tauto.
+  + intros.
+    rewrite Same_set_spec in H4; rewrite (H4 n), Union_spec in H5.
+    rewrite Same_set_spec in H3; specialize (H3 n).
+    rewrite Intersection_spec in H3.
+    unfold unmarked', unmarked, Complement, Ensembles.In in H3.
+    rewrite Intersection_spec, !negateP_spec in H3.
+    destruct (node_pred_dec (marked g1) n), (node_pred_dec (marked g) n); destruct_eq_dec root n; tauto.
+Qed.
+
+Lemma mark1_mark_list_mark: forall root l (g1 g2: Graph),
   vvalid g1 root ->
   (unmarked g1) root ->
   step_list g1 root l ->
@@ -217,6 +323,29 @@ Lemma mark1_mark_list_mark: forall root l (g1 g2: Graph)
   mark root g1 g2.
 Proof.
   intros.
+  rename g1 into g.
+  destruct_relation_list g1 in H2.
+  pose proof triple_mark1 root g g1 H3.
+  cbv zeta in H4.
+  set (unmarked' := Intersection _ (unmarked g) (Complement _ (eq root))) in H4.
+  set (PV1 := reachable_by_through_set g nil unmarked') in H4.
+  set (PV2 := reachable_by_through_set g l unmarked').
+  assert ((predicate_partialgraph g (Complement V PV2)) ~=~
+          (predicate_partialgraph g2 (Complement V PV2)) /\
+          Same_set (unmarked g2) (Intersection V unmarked' (Complement V PV2)));
+  [| eapply triple_final; eauto].
+  clear H3.
+
+  set (l_done := l).
+  set (l_later := @nil V).
+  assert (l = l_done ++ l_later) by (unfold l_later; rewrite app_nil_r; auto).
+  revert PV2 H2; change l with l_done; intros.
+  clearbody l_done l_later.
+  revert l_later H3; induction l_done; intros.
+  + unfold mark_list, relation_list in H2.
+    simpl in H2; subst g2.
+    auto.
+  + clear PV1 H4.
 Admitted.
 
 Lemma vertex_update_mark1: forall (g: Graph) x lx,
@@ -233,7 +362,8 @@ Proof.
     unfold update_vlabel.
     destruct_eq_dec x n'; [tauto | auto].
   + simpl; intros.
-    auto.
+    unfold update_vlabel in H1.
+    destruct_eq_dec x n'; [tauto | auto].
 Qed.
 
 (*
